coq/Completeness.v
@@ -61,6 +61,18 @@ Definition dynamic_int_by_sort s (n : smt_sort_to_int_type s) : dynamic_int :=
   f n
 .
 
+Lemma eval_udiv_correspondence : forall m s (ast : smt_ast s) n,
+  (n <> 0)%Z ->
+  over_approx_via_model
+    (eval_ibinop
+      (UDiv false)
+      (DV_Int (dynamic_int_by_sort s (smt_eval_ast m s ast)))
+      (DV_Int (dynamic_int_by_sort s (repr_by_sort s n))))
+    (Some (Expr s (AST_BinOp s SMT_UDiv ast (AST_Const s (repr_by_sort s n)))))
+    m.
+Proof.
+Admitted.
+
 Lemma eval_shl_correspondence : forall m s (ast : smt_ast s) n,
   (n >= 0)%Z ->
   (n < Zpos (smt_sort_to_width s))%Z ->
@@ -423,9 +435,11 @@ Proof.
         inversion H4; subst.
         rename sort into sort1, ast into ast1, sort0 into sort2, ast0 into ast2.
         destruct op;
-        try inversion H5; (
-          destruct sort1, sort2; try (apply OA_None); (
-            eapply OA_Some; reflexivity
+        try (
+          inversion H5; (
+            destruct sort1, sort2; try (apply OA_None); (
+              eapply OA_Some; reflexivity
+            )
           )
         ).
       }
@@ -437,6 +451,49 @@ Proof.
     }
     {
       inversion H2; subst.
+      apply OA_None.
+    }
+  }
+  {
+    apply IHe1 with (ot := (Some t)) in H4.
+    assert(L: is_supported_exp (EXP_Integer n)).
+    { apply IS_EXP_Integer. }
+    apply IHe2 with (ot := (Some t)) in L.
+    destruct (eval_exp c_ls c_gs (Some t) e1) as [dv1 | ] eqn:E1.
+    {
+      destruct (eval_exp c_ls c_gs (Some t) (EXP_Integer n)) as [dv2 | ] eqn:E2.
+      {
+        inversion H2; subst.
+        {
+          simpl.
+          inversion H4; subst.
+          inversion L; subst.
+          rename sort into sort1, ast into ast1, sort0 into sort2, ast0 into ast2.
+          destruct t; try discriminate H1.
+          assert(Lw : w = (smt_sort_to_width sort2)).
+          { apply infer_width in H1. assumption. }
+          destruct sort1, sort2; try (apply OA_None);
+          (
+            subst;
+            simpl in H1;
+            inversion H1; subst;
+            apply inj_pair2 in H3;
+            subst;
+            apply eval_udiv_correspondence;
+            assumption
+          ).
+        }
+      }
+      {
+        inversion H4; subst.
+        inversion L; subst.
+        simpl.
+        rewrite <- H.
+        apply OA_None.
+      }
+    }
+    {
+      inversion H4; subst.
       apply OA_None.
     }
   }
